src/Hlist.v
@@ -1,0 +1,69 @@
+Require Import List.
+Import List.ListNotations.
+Open Scope list.
+
+Set Implicit Arguments.
+
+Section hlist.
+  Variable A : Type.
+  Variable B : A -> Type.
+
+  Inductive hlist : list A -> Type :=
+  | HNil : hlist nil
+  | HCons : forall (a:A) (types: list A), B a -> hlist types -> hlist (a::types).
+
+  Variable elm : A.
+
+  Inductive member : list A -> Type :=
+  | HFirst : forall types, member (elm :: types)
+  | HNext : forall a types, member types -> member (a::types).
+
+  (** Adapted from CPDT DataStruct hlist.
+
+      In Coq v8.5beta2 at least, the return annotations are unnecessary. *)
+  Fixpoint get types (l: hlist types) : member types -> B elm :=
+    match l with
+    | HNil => fun mem =>
+               match mem in member ls' return (match ls' with
+                                               | nil => B elm
+                                               | _ :: _ => unit
+                                               end) with
+               | HFirst _ => tt
+               | HNext _ _ => tt
+               end
+    | HCons x mls' => fun mem =>
+                       match mem in member ls' return (match ls' with
+                                                       | nil => Empty_set
+                                                       | x' :: ls'' =>
+                                                         B x' -> (member ls'' -> B elm)
+                                                         -> B elm
+                                                       end) with
+                       | HFirst _ => fun x _ => x
+                       | HNext _ mem' => fun _ get_mls' => get_mls' mem'
+                       end x (get mls')
+    end.
+
+  Fixpoint set types (l: hlist types) (new: B elm) : member types -> (hlist types) :=
+    match l with
+    | HNil => fun mem => HNil
+    | HCons x mls' => fun mem =>
+                       match mem in member ls' with
+                       | HFirst _ => fun x _ => HCons new mls'
+                       | HNext _ mem' => fun x set_mls' => HCons x (set_mls' mem')
+                       end x (set mls' new)
+    end.
+
+End hlist.
+
+Arguments HCons [A] [B] [a] [types] el xs.
+Arguments HNil [A] [B].
+Arguments HFirst [A] [elm] [types].
+Arguments HNext [A] [elm] [a] [types] mem.
+
+Example types := [nat; bool; nat].
+Example someValues : hlist (fun T : Set => T) types := HCons 5 (HCons true (HCons 3 HNil)).
+
+Eval simpl in get someValues HFirst.
+Eval simpl in get someValues (HNext HFirst).
+
+Eval simpl in set someValues false (HNext HFirst).
